Need to prove termination of compare

michael_formal/EFSM.thy
@@ -45,9 +45,46 @@ primrec observe_trace :: "efsm \<Rightarrow> statename \<Rightarrow> registers \
     )"
 declare observe_trace_def [simp]
 
+definition equiv :: "efsm \<Rightarrow> efsm \<Rightarrow> trace \<Rightarrow> bool" where
+  "equiv e1 e2 t \<equiv> ((observe_trace e1 (s0 e1) <> t) = (observe_trace e2 (s0 e2) <> t))"
+declare equiv_def [simp]
 
+lemma equiv_comute: "equiv e1 e2 t \<equiv> equiv e2 e1 t"
+  apply simp
+  by argo
 
+lemma equiv_trans: "equiv e1 e2 t \<and> equiv e2 e3 t \<longrightarrow> equiv e1 e3 t"
+  by simp
 
+lemma equiv_idem: "equiv e1 e1 t"
+  by simp
 
+definition all_outs :: "efsm \<Rightarrow> statename \<Rightarrow> destination list" where
+  "all_outs e s = [(s',t) . s' \<leftarrow> S e, t \<leftarrow> T e(s,s'), (find (\<lambda>x . x = t) (T e(s,s')) \<noteq> None)]"
+
+definition can_take :: "transition \<Rightarrow> transition \<Rightarrow> bool" where
+  "can_take t1 t2 \<equiv> ((Label t1) = (Label t2)) \<and> ((Arity t1) = (Arity t2))"
+
+primrec find_match :: "transition \<Rightarrow> destination list \<Rightarrow> destination option" where
+  "find_match _ [] = None" |
+  "find_match t (h#tail) = (if (can_take t (snd h)) then (Some h) else (find_match t tail))"
+
+fun match_all :: "efsm \<Rightarrow> (string, bexp) map \<Rightarrow> destination list \<Rightarrow> efsm \<Rightarrow> (string, bexp) map \<Rightarrow> destination list \<Rightarrow> statename list \<Rightarrow> bool" 
+  and compare :: "efsm \<Rightarrow> statename \<Rightarrow> (string, bexp) map \<Rightarrow> efsm \<Rightarrow> statename \<Rightarrow> (string, bexp) map \<Rightarrow> statename list \<Rightarrow> bool" 
+  where
+  "match_all _ _ [] _ _ _ _ = True" |
+  "match_all e1 c1 (h#t) e2 c2 d2 closed = (
+    case (find_match (snd h) d2) of
+      None \<Rightarrow> False  |
+      Some (s', _) \<Rightarrow> (compare e1 (fst h) c1 e2 s' c2 closed ) \<and> (match_all e1 c1 t e2 c2 d2 closed)
+    )" |
+ "compare  e1 s1 c1 e2 s2 c2 closed = (
+    if ((find (\<lambda>x . x = s1) closed) \<noteq> None) then
+      True
+    else (match_all e1 c1 (all_outs e1 s1) e2 c2 (all_outs e2 s2) (s1#closed)
+     ))"
+
+definition simulates :: "efsm \<Rightarrow> efsm \<Rightarrow> bool" where
+  "simulates e1 e2 = compare e1 (s0 e1) empty e2 (s0 e2) empty []"
 
 end
