michael_formal/types.thy
@@ -20,6 +20,8 @@ record transition =
   Outputs :: "output_function"
   Updates :: "update_function"
 
+type_synonym destination = "(statename \<times> transition)"
+
 record efsm =
   S :: "statename list"
   s0 :: "statename"
